CodeGen.v
@@ -25,6 +25,7 @@ Require Import PolyLoop.
 Require Import PolyLoopSimpl.
 Require Import LoopGen.
 Require Import Loop.
+Require Import Misc.
 
 Open Scope Z_scope.
 
@@ -50,24 +51,51 @@ Qed.
 
 
 
-Definition complete_generate_many d n pis :=
+Definition complete_generate_lex_many d n pis :=
   BIND polyloop <- generate_loop_many d n pis -;
   BIND simp <- polyloop_simplify polyloop (n - d)%nat nil -;
   polyloop_to_loop (n - d)%nat simp.
 
-Theorem complete_generate_many_preserve_sem :
+Theorem complete_generate_lex_many_preserve_sem :
   forall d n pis env mem1 mem2,
     (d <= n)%nat ->
-    WHEN st <- complete_generate_many d n pis THEN
+    WHEN st <- complete_generate_lex_many d n pis THEN
     loop_semantics st env mem1 mem2 ->
     length env = (n - d)%nat ->
     pis_have_dimension pis n ->
     env_poly_lex_semantics (rev env) n pis mem1 mem2.
 Proof.
   intros d n pis env mem1 mem2 Hdn st Hst Hloop Henv Hpis.
-  unfold complete_generate_many in Hst.
+  unfold complete_generate_lex_many in Hst.
   bind_imp_destruct Hst polyloop Hpolyloop; bind_imp_destruct Hst simp Hsimp.
   eapply generate_loop_many_preserves_sem; eauto; [|unfold generate_invariant; auto].
   eapply polyloop_simplify_correct; [|exact Hsimp| | |]; auto; [unfold poly_nrl; simpl; lia|].
   eapply polyloop_to_loop_correct; eauto.
+Qed.
+
+Definition complete_generate_many es n pis :=
+  let k := list_max (map (fun pi => length pi.(pi_schedule)) pis) in
+  let epis := elim_schedule k es pis in
+  complete_generate_lex_many (n + k - es)%nat (n + k)%nat epis.
+
+Theorem complete_generate_many_preserve_sem :
+  forall es n pis env mem1 mem2,
+    (es <= n)%nat ->
+    WHEN st <- complete_generate_many es n pis THEN
+    loop_semantics st env mem1 mem2 ->
+    length env = es ->
+    pis_have_dimension pis n ->
+    (forall pi, In pi pis -> (poly_nrl pi.(pi_schedule) <= n)%nat) ->
+    env_poly_semantics (rev env) n pis mem1 mem2.
+Proof.
+  intros es n pis env mem1 mem2 Hes st Hst Hloop Henv Hpis Hpis2.
+  unfold complete_generate_many in Hst.
+  eapply complete_generate_lex_many_preserve_sem in Hst; [|lia].
+  eapply poly_elim_schedule_semantics_env_preserve; [| |apply Hst|]; auto; try lia.
+  - rewrite rev_length; auto.
+  - unfold pis_have_dimension, elim_schedule in *. rewrite forallb_map, forallb_forall in *.
+    intros pi Hpi; specialize (Hpis pi Hpi). reflect.
+    rewrite pi_elim_schedule_nrl by (apply list_max_ge; rewrite in_map_iff; exists pi; auto).
+    specialize (Hpis2 pi Hpi); lia.
+  - intros k pi Hpi. apply nth_error_In in Hpi. apply list_max_ge. rewrite in_map_iff; exists pi; auto.
 Qed.
